Start working on a more general equivalence relation for expressions

Source/DafnyCompilers/CompilerCommon.dfy
@@ -24,15 +24,15 @@ module {:extern "DafnyInDafny.Common"} DafnyCompilerCommon {
 
       type Path = seq<string>
 
-      datatype ClassType = ClassType(className: Path, typeArgs: seq<Type>)
+      datatype ClassType = ClassType(className: Path, typeArgs: seq<TypeRaw>)
 
       datatype CollectionKind =
         | Seq
         | Set
         | Multiset
-        | Map(keyType: Type)
+        | Map(keyType: TypeRaw)
 
-      datatype Type =
+      datatype TypeRaw =
         | Unit
         | Bool
         | Char
@@ -40,9 +40,69 @@ module {:extern "DafnyInDafny.Common"} DafnyCompilerCommon {
         | Real
         | BigOrdinal
         | BitVector(width: nat)
-        | Collection(finite: bool, kind: CollectionKind, eltType: Type)
-        | Function(args: seq<Type>, ret: Type) // TODO
+        | Collection(finite: bool, kind: CollectionKind, eltType: TypeRaw)
+        | Function(args: seq<TypeRaw>, ret: TypeRaw) // TODO
         | Class(classType: ClassType)
+      {
+        // No function/class appear in the type 
+        predicate method NoFunction() {
+          match this {
+            case Unit => true
+            case Bool => true
+            case Char => true
+            case Int => true
+            case Real => true
+            case BigOrdinal => true
+            case BitVector(width: nat) => true
+            case Collection(finite: bool, kind: CollectionKind, eltType: TypeRaw) =>
+              && eltType.NoFunction()
+              && match kind {
+                case Map(kt) => kt.NoFunction() // TODO: redundant branch if I put it below??
+                case Seq => true
+                case Set => true
+                case MultiSet => true
+              }
+            case Function(args: seq<TypeRaw>, ret: TypeRaw) => false
+            case Class(classType: ClassType) => false
+          }
+        }
+
+        // TODO: TranslateType doesn't fail after I added this condition to Type, I don't understand why.
+        // I see that TranslateType never returns Function or Class, but there is still a bit of magic...
+        predicate method WellFormed() {
+          match this {
+            case Unit => true
+            case Bool => true
+            case Char => true
+            case Int => true
+            case Real => true
+            case BigOrdinal => true
+            case BitVector(width: nat) => true
+            case Collection(finite: bool, kind: CollectionKind, eltType: TypeRaw) =>
+              && eltType.WellFormed()
+              // This condition is overly restrictive: we will do the general case later.
+              // The more general condition would be that keys can't contain functions.
+              // Note that collections like sequences and maps have (or not) a decidable
+              // equality depending on whether their elements have a decidable equality or
+              // not. We might want to enforce that in the future (we would need to have
+              // more well-formedness conditions on the expressions).
+              && eltType.NoFunction()
+              && match kind {
+                case Map(kt) => kt.WellFormed() && kt.NoFunction() // TODO: redundant branch if I put it below??
+                case Seq => true
+                case Set => eltType.NoFunction()
+                case MultiSet => eltType.NoFunction()
+              }
+            case Function(args: seq<TypeRaw>, ret: TypeRaw) =>
+              && (forall i | 0 <= i < |args| :: args[i].WellFormed())
+              && ret.WellFormed()
+            case Class(classType: ClassType) =>
+              && (forall i | 0 <= i < |classType.typeArgs| :: classType.typeArgs[i].WellFormed())
+          }
+        }
+      }
+      
+      type Type(!new,00,==) = ty:TypeRaw | ty.WellFormed() witness Unit
 
       type T(!new,00,==) = Type
     }
